Working towards wf_ctx

src/Coq/env.v
@@ -32,7 +32,7 @@ Definition Dom {A:Type} (m: env A):= map fst m.
 Definition wf_extd {A: Type} (m:env A) xs := (forall x, In x xs -> ~In x (Dom m)) /\ (NoDup xs).
 *)
 Inductive wf_extd {A: Type} (m:env A) xs : Prop :=
-  | wf_extds : forall x, In x xs -> ~In x (Dom m) -> NoDup xs -> wf_extd m xs.
+  | wf_extds : (forall x, In x xs -> ~In x (Dom m)) -> NoDup xs -> wf_extd m xs.
 
 Lemma update_not_shadow: forall {A: Type} (m: env A) x a,
   In x (Dom m) ->
@@ -44,6 +44,12 @@ Proof.
   case beq_id; auto.
   rewrite IHm; auto.
 Qed.
+
+Lemma extds_not_shadow: forall {A: Type} xs (m: env A) x bs,
+  In x (Dom m) ->
+  get (m extds xs : bs) x = get m x.
+Proof.
+Admitted.
 
 
 Theorem extend_neq : forall (X:Type) (m : env X) v x1 x2,
@@ -133,32 +139,144 @@ Lemma get_wf_extd: forall (A: Type) (m: env A) x b i,
 Proof.
 Admitted.
 Print combine.
+
+(*
 Lemma extds_nil: forall (B: Type) (xs: list id) (bs: list B),
   @wf_extd id nil xs ->
   [] extds xs : bs = combine xs bs.
 Proof.
   induction xs, bs; simpl; auto.
-  intros. destruct H. simpl in *. 
-  destruct H; inversion H1; subst. 
+  intros. destruct H. simpl in *.  
+  edestruct H. inversion H1. esubst. 
+Admitted.
+*)
 
-admit.
-  
-  inversion H0. 
-  unfold extend_list. 
-  simpl.
-  simpl.
+Lemma get_noteq: forall (A:Type) (m: env A) x' x a,
+  x' <> x ->
+  get ((x', a) :: m) x = get m x.
+Proof.
+  induction m.
+  intros; simpl; auto.
+  rewrite not_eq_beq_id_false; auto.
+  intros. simpl.
+  rewrite not_eq_beq_id_false; auto.
+Qed.
 
-Theorem get_wf_extds: forall (A: Type) (m: env A) xs bs x b i,
+Lemma get_in_Dom: forall (A: Type) (b: A) m x,
+  get m x = Some b ->
+  In x (Dom m).
+Proof.
+  induction m.
+  intros. inversion H.
+  destruct a.
+  intros.
+  unfold Dom. simpl.
+  destruct eq_id_dec with x i. left; auto.
+  right.
+  apply IHm.
+  rewrite get_noteq in H; auto.
+Qed.
+
+
+Lemma in_notin_noteq: forall {A:Type} xs (x1: A) x2,
+  In x1 xs ->
+  ~In x2 xs ->
+  x1 <> x2.
+Proof.
+  induction xs.
+  intros; inversion H.
+  intros.
+  simpl in *.
+  apply Decidable.not_or in H0. destruct H0.
+  destruct H.
+  rewrite <- H; auto.
+  apply IHxs; auto.
+Qed.
+
+Lemma wf_weak: forall (A:Type) (m: env A) (x: id) xs,
+  wf_extd m (x::xs) ->
+  wf_extd m xs.
+Proof.
+  induction m.
+  intros. destruct H.
+  constructor; auto. intros.
+  inversion H0; auto.
+  destruct a; intros.
+  constructor.
+  intros.
+  simpl.
+  intro.
+  destruct H. destruct H1. eapply H.
+  simpl. right. apply H0.
+  rewrite H1; simpl; auto.
+  eapply H. simpl. right. exact H0.
+  simpl. right; auto.
+  destruct H. inversion H0; auto.
+Qed.
+
+
+Lemma get_extd_notin_Dom: forall (A: Type) (b0: A) m x xs bs,
+  ~In x (Dom m) ->
+  get (m extds (x::xs) : (b0 ::bs)) x = Some b0.
+Proof.
+  induction m. simpl.
+  intros. rewrite extds_not_shadow. simpl. rewrite beq_id_refl. auto.
+  simpl; auto. 
+  destruct a; simpl; auto.
+  simpl in *.
+  SearchAbout not or. intros.
+  apply Decidable.not_or in H. destruct H.
+  rewrite not_eq_beq_id_false; auto.
+Admitted.
+
+
+Lemma get_extds_notin_head: forall (A: Type) (m: env A) xs bs x' x b,
+  x <> x' ->
+  get (m extds (x':: xs) : (b::bs)) x = get (m extds xs : bs) x.
+Proof.
+  intros; simpl.
+Admitted.
+
+Theorem get_wf_extds: forall (A: Type)  xs (m: env A) bs x b i,
   wf_extd m xs ->
   get (m extds xs : bs) x = Some b ->
   nth_error xs i = Some x ->
   nth_error bs i = Some b.
 Proof.
-  induction m; intros.
-  Case "[]".
-    unfold extend_list in H0. 
-    simpl in *.
- unfold wf_extd in *. simpl in H.
-    intros.
+  induction xs. 
+  intros. inversion H. rewrite nth_error_nil in H1. inversion H1.
   intros.
-Admitted.
+  destruct H.
+  inversion H2.
+  assert (i=0).
+    eapply nth_error_fst. exact H2. rewrite <- H3 in H1; auto.
+  case bs in *. simpl in H0. 
+  apply get_in_Dom in H0.
+  false. apply H with x; auto. rewrite <- H3. apply nth_error_In with i;auto.
+  subst.
+  
+  rewrite H6; simpl.
+  rewrite H5 in H0.
+  rewrite get_extd_notin_Dom in H0; auto.
+
+  case i in *.
+  case bs in *. simpl in H0.
+  apply get_in_Dom in H0. contradiction.
+  simpl in *.
+  inversion H1. rewrite H7 in H2.
+  inversion H2. subst. contradiction.
+  
+  case bs in *.
+  simpl in *. 
+  apply get_in_Dom in H0; contradiction.
+  inversion H2. subst.
+  
+  simpl in *.
+  eapply in_notin_noteq in H5; eauto.
+  apply IHxs with m x; auto.
+  apply wf_weak with a.
+  constructor; auto.
+
+  erewrite <- get_extds_notin_head; eauto.
+
+Qed.
